Replace `fresh` with weaker `dead`
We now require, at level 0, that any dead location be disjoint
from any live location of the same memory state. This is still
generalizable to any level.

This is necessary to support deallocation of individual
references (as opposed to deallocating a whole region, which
was already supported.)

ulib/FStar.Modifies.fst
@@ -127,20 +127,18 @@ let level_0_class_eq_root_t
 = squash (level == 0 ==> ty == root_type /\ c == root_class)
 
 unfold
-let level_0_fresh_disjoint_t
+let level_0_live_dead_disjoint_t
   (#heap: Type u#a)
   (#level: nat) (#ty: Type u#b) (c: class' heap level ty)
 : Tot (Type u#(max a b))
 = (oold: ty) ->
   (onew: ty) ->
   (hbefore: heap) ->
-  (hafter: heap) ->
   Lemma
   (requires (
     level == 0 /\
     Class?.live c hbefore oold /\
-    (~ (Class?.contains c hbefore onew)) /\
-    Class?.live c hafter onew
+    (~ (Class?.contains c hbefore onew))
   ))
   (ensures (Class?.disjoint c oold onew))
 
@@ -355,7 +353,7 @@ type class_invariant_body
   preserved_ancestors_preserved: preserved_ancestors_preserved_t c;
   disjoint_sym: disjoint_sym_t c;
   level_0_class_eq_root: level_0_class_eq_root_t root_class c;
-  level_0_fresh_disjoint: level_0_fresh_disjoint_t c;
+  level_0_live_dead_disjoint: level_0_live_dead_disjoint_t c;
   live_preserved_preserved: live_preserved_preserved_t c;
   preserved_live: preserved_live_t c;
   preserved_contains: preserved_contains_t c;
@@ -510,22 +508,20 @@ let level_0_class_eq_root
 = Squash.bind_squash #_ #(0 == 0 ==> ty == root_type /\ c == root_class) (Squash.join_squash ()) (fun (i: class_invariant_body root_class c) -> i.level_0_class_eq_root)
 
 abstract
-let level_0_fresh_disjoint
+let level_0_live_dead_disjoint
   (#heap: Type u#a)
   (#root_type: Type u#b) (root_class: class' heap 0 root_type { class_invariant root_class root_class } )
   (oold: root_type)
   (onew: root_type)
   (hbefore: heap)
-  (hafter: heap)
 : Lemma
   (requires (
     Class?.live root_class hbefore oold /\
-    (~ (Class?.contains root_class hbefore onew)) /\
-    Class?.live root_class hafter onew
+    (~ (Class?.contains root_class hbefore onew))
   ))
   (ensures (Class?.disjoint root_class oold onew))
-  [SMTPatT u#c (Class?.live root_class hbefore oold); SMTPatT (~ (Class?.contains root_class hbefore onew)); SMTPatT (Class?.live root_class hafter oold); SMTPatT (Class?.live root_class hafter onew)]
-= Squash.bind_squash #_ #(Class?.disjoint root_class oold onew) (Squash.join_squash ()) (fun (i: class_invariant_body root_class root_class) -> i.level_0_fresh_disjoint oold onew hbefore hafter)
+  [SMTPatT u#c (Class?.live root_class hbefore oold); SMTPatT (~ (Class?.contains root_class hbefore onew)); ]
+= Squash.bind_squash #_ #(Class?.disjoint root_class oold onew) (Squash.join_squash ()) (fun (i: class_invariant_body root_class root_class) -> i.level_0_live_dead_disjoint oold onew hbefore)
 
 abstract
 let live_preserved_preserved
@@ -1278,62 +1274,37 @@ let modifies_test_1
   (ensures (Class?.preserved c o3 h h'))
 = ()
 
-let rec fresh
+let rec dead
   (#heap: Type u#a)
   (#level: nat)
   (#ty: Type u#b)
   (c: class' heap level ty)
   (o: ty)
-  (h h': heap)
+  (h: heap)
 : Pure Type0
   (requires True)
   (ensures (fun _ -> True))
   (decreases level)
-= (~ ( Class?.contains c h o )) /\
-  Class?.live c h' o /\ (
-    forall (i: nat {i < Class?.ancestor_count c o}) . fresh (Class?.ancestor_classes c o i) (Class?.ancestor_objects c o i) h h'
+= (~ ( Class?.contains c h o )) /\ (
+    forall (i: nat {i < Class?.ancestor_count c o}) . dead (Class?.ancestor_classes c o i) (Class?.ancestor_objects c o i) h
   )
 
-let fresh_ancestor
+let dead_ancestor
   (#heap: Type u#a)
   (#level: nat)
   (#ty: Type u#b)
   (c: class' heap level ty)
   (o: ty)
-  (h h': heap)
+  (h: heap)
   (i: nat {i < Class?.ancestor_count c o})
 : Lemma
-  (requires (fresh c o h h'))
-  (ensures (fresh (Class?.ancestor_classes c o i) (Class?.ancestor_objects c o i) h h'))
-  [SMTPat (fresh (Class?.ancestor_classes c o i) (Class?.ancestor_objects c o i) h h')]
+  (requires (dead c o h))
+  (ensures (dead (Class?.ancestor_classes c o i) (Class?.ancestor_objects c o i) h))
+  [SMTPat (dead (Class?.ancestor_classes c o i) (Class?.ancestor_objects c o i) h)]
 = ()
 
 abstract
-let rec fresh_live
-  (#heap: Type u#a)
-  (#root_type: Type u#b) (#root_class: class' heap 0 root_type)
-  (#level: nat)
-  (#ty: Type u#b)
-  (c: class root_class level ty)
-  (o: ty)
-  (h0 h1 h2: heap)
-: Lemma
-  (requires (fresh c o h0 h1 /\ Class?.live c h2 o))
-  (ensures (fresh c o h0 h2))
-  [SMTPatT u#c (fresh c o h0 h1); SMTPatT (Class?.live c h2 o)]
-= let f
-    (i: nat {i < Class?.ancestor_count c o})
-  : Lemma
-    (ensures (
-      fresh (Class?.ancestor_classes c o i) (Class?.ancestor_objects c o i) h0 h2
-    ))
-  = let (c': class root_class (Class?.ancestor_class_levels c o i) (Class?.ancestor_types c o i)) = (Class?.ancestor_classes c o i) in
-    fresh_live c' (Class?.ancestor_objects c o i) h0 h1 h2
-  in
-  Classical.forall_intro f
-
-abstract
-let rec fresh_disjoint
+let rec live_dead_disjoint
   (#heap: Type u#a)
   (#root_type: Type u#b) (#root_class: class' heap 0 root_type)
   (#levelold: nat) (#tyold: Type u#b)
@@ -1343,15 +1314,14 @@ let rec fresh_disjoint
   (oold: tyold)
   (onew: tynew)
   (hbefore: heap)
-  (hafter: heap)
 :  Lemma
   (requires (
     Class?.live cold hbefore oold /\
-    fresh cnew onew hbefore hafter
+    dead cnew onew hbefore
   ))
   (ensures (loc_disjoint (loc_of_object cold oold) (loc_of_object cnew onew)))
   (decreases (levelold + levelnew))
-  [SMTPatT u#c (Class?.live cold hbefore oold); SMTPatT (fresh cnew onew hbefore hafter)]
+  [SMTPatT u#c (Class?.live cold hbefore oold); SMTPatT (dead cnew onew hbefore)]
 = if
     levelold = 0
   then
@@ -1360,7 +1330,7 @@ let rec fresh_disjoint
       levelnew = 0
     then
       let _ : squash (tynew == root_type /\ cnew == root_class) = level_0_class_eq_root #heap #root_type #root_class #tynew cnew in
-      level_0_fresh_disjoint cold oold onew hbefore hafter
+      level_0_live_dead_disjoint cold oold onew hbefore
     else
       let f
 	(i: nat { i < Class?.ancestor_count cnew onew } )
@@ -1368,7 +1338,7 @@ let rec fresh_disjoint
 	(loc_disjoint (loc_of_object cold oold) (loc_of_object (Class?.ancestor_classes cnew onew i) (Class?.ancestor_objects cnew onew i)))
       = let cnew' = Class?.ancestor_classes cnew onew i in
 	let onew' = Class?.ancestor_objects cnew onew i in
-	fresh_disjoint cold cnew' oold onew' hbefore hafter
+	live_dead_disjoint cold cnew' oold onew' hbefore
       in
       loc_disjoint_ancestors_right (loc_of_object cold oold) cnew onew f
   else
@@ -1378,7 +1348,7 @@ let rec fresh_disjoint
       (loc_disjoint (loc_of_object (Class?.ancestor_classes cold oold i) (Class?.ancestor_objects cold oold i)) (loc_of_object cnew onew))
     = let cold' = Class?.ancestor_classes cold oold i in
       let oold' = Class?.ancestor_objects cold oold i in
-      fresh_disjoint cold' cnew oold' onew hbefore hafter
+      live_dead_disjoint cold' cnew oold' onew hbefore
     in
     loc_disjoint_ancestors_left cold oold (loc_of_object cnew onew) f
 
@@ -1450,28 +1420,27 @@ let locset_live
   TSet.mem (loc_of_object c o) ls ==>
   Class?.live c h o
 
-let locset_fresh
+let locset_dead
   (#heap: Type u#a)
   (#root_type: Type u#b)
   (#root_class: class' heap 0 root_type)
   (ls: locset root_class)
-  (h h': heap)
+  (h: heap)
 : Tot Type0
 = forall (level: nat) (ty: Type u#b) (c: class root_class level ty) (o: ty) .
   TSet.mem (loc_of_object c o) ls ==>
-  fresh c o h h'
+  dead c o h
 
 abstract
-let locset_fresh_locset_disjoint
+let locset_live_locset_dead_locset_disjoint
   (#heap: Type u#a)
   (#root_type: Type u#b) (#root_class: class' heap 0 root_type)
   (lsold lsnew: locset root_class)
   (hbefore: heap)
-  (hafter: heap)
 : Lemma
   (requires (
     locset_live hbefore lsold /\
-    locset_fresh lsnew hbefore hafter
+    locset_dead lsnew hbefore
   ))
   (ensures (locset_disjoint lsold lsnew))
 = let f
@@ -1479,18 +1448,18 @@ let locset_fresh_locset_disjoint
     (lnew: loc root_class { TSet.mem lnew lsnew } )
   : Lemma
     (loc_disjoint lold lnew)
-  = fresh_disjoint (Location?.class lold) (Location?.class lnew) (Location?.obj lold) (Location?.obj lnew) hbefore hafter
+  = live_dead_disjoint (Location?.class lold) (Location?.class lnew) (Location?.obj lold) (Location?.obj lnew) hbefore
   in
   Classical.forall_intro_2 f
 
-let modifies_fresh_elim
+let modifies_locset_dead
   (#heap: Type u#a)
   (#root_type: Type u#b) (#root_class: class' heap 0 root_type)
   (lsold lsnew: locset root_class)
   (hbefore: heap)
   (hafter: heap)
 : Lemma
-  (requires (modifies (TSet.union lsold lsnew) hbefore hafter /\ locset_fresh lsnew hbefore hafter))
+  (requires (modifies (TSet.union lsold lsnew) hbefore hafter /\ locset_dead lsnew hbefore))
   (ensures (modifies lsold hbefore hafter))
 = let f'
     (ty: Type u#b)
@@ -1516,7 +1485,7 @@ let modifies_fresh_elim
         (fun _ -> g o')
         (fun _ ->
           let (Location _ _ cnew onew) = o' in
-          fresh_disjoint c cnew o onew hbefore hafter
+          live_dead_disjoint c cnew o onew hbefore
         )
     in
     modifies_elim (TSet.union lsold lsnew) hbefore hafter () c o g'
